Refactor IPDA to only allow transitions where the items are in It G'. Continue proofs

Escallon/LR_Parsing/Item_Pushdown_Automata.thy
@@ -8,14 +8,15 @@ definition (in Extended_Cfg) IPDA :: "(('n, 't) item, 't, ('n, 't) item) pda" wh
   "IPDA \<equiv> let
     P = Prods G';
     \<Delta> = (\<lambda>q a s. case q of [X \<rightarrow> \<beta> . Tm a' # \<gamma>] \<Rightarrow> 
-            if a' = a then let r = [X \<rightarrow> \<beta> @ [Tm a] . \<gamma>] in {(r, [s])} else {} | _ \<Rightarrow> {});
-    \<E> = (\<lambda>q s. case (q,s) of 
-      ([X \<rightarrow> \<beta> . Nt Y # \<gamma>], _) \<Rightarrow> {([Y \<rightarrow> [] . \<alpha>], [X \<rightarrow> \<beta> . Nt Y#\<gamma>]#[s]) |\<alpha>. (Y,\<alpha>) \<in> P} |
+            if a' = a \<and> (X, \<beta> @ Tm a' # \<gamma>) \<in> P then let r = [X \<rightarrow> \<beta> @ [Tm a] . \<gamma>] in {(r, [s])} 
+        else {} | _ \<Rightarrow> {});
+    \<E> = (\<lambda>q s. if prod_of_item q \<notin> P then {} else case (q,s) of 
+      ([X \<rightarrow> \<beta> . Nt Y # \<gamma>], _) \<Rightarrow> 
+        {([Y \<rightarrow> [] . \<alpha>], [X \<rightarrow> \<beta> . Nt Y#\<gamma>]#[s]) |\<alpha>. (Y,\<alpha>) \<in> P} |
       ([Y \<rightarrow> \<alpha> . []], [X \<rightarrow> \<beta> . Nt Y' # \<gamma>]) 
-        \<Rightarrow> if Y = Y' then {([X \<rightarrow> \<beta>@[Nt Y] . \<gamma>], [])} else {} | _ \<Rightarrow> {})         
-in
-  \<lparr>init_state = [S' \<rightarrow> [] . [Nt S]], init_symbol = [S' \<rightarrow> [] . []], 
-    final_states = {[S' \<rightarrow> [Nt S] . []]}, delta = \<Delta>, delta_eps = \<E>\<rparr>"
+        \<Rightarrow> if Y = Y' \<and> prod_of_item s \<in> P then {([X \<rightarrow> \<beta>@[Nt Y] . \<gamma>], [])} else {} | _ \<Rightarrow> {})         
+  in \<lparr>init_state = [S' \<rightarrow> [] . [Nt S]], init_symbol = [S' \<rightarrow> [] . []], 
+      final_states = {[S' \<rightarrow> [Nt S] . []]}, delta = \<Delta>, delta_eps = \<E>\<rparr>"
 
 
 locale ipda = Extended_Cfg G for G :: "('n::fresh0, 't) Cfg" +
@@ -26,11 +27,11 @@ begin
 
 lemma init_state_ipda [simp]:
   "init_state M = [S' \<rightarrow> [] . [Nt S]]"
-  using ipda unfolding IPDA_def by simp
+  using ipda unfolding IPDA_def by (meson select_convs(1))
 
 lemma init_symbol_ipda [simp]:
   "init_symbol M = [S' \<rightarrow> [] . []]"
-  using ipda unfolding IPDA_def by simp
+  using ipda unfolding IPDA_def by (meson select_convs(2))
 
 lemma init_symbol_notin_It: 
   "init_symbol M \<notin> It G'"
@@ -52,19 +53,17 @@ abbreviation "final_state \<equiv> [S' \<rightarrow> [Nt S] . []]"
 
 lemma final_states_ipda [simp]:
   "final_states M = {final_state}"
-  using ipda unfolding IPDA_def by simp
+  using ipda unfolding IPDA_def by (meson select_convs(3))
+
+lemma final_state_in_It [simp]:
+  "final_state \<in> It G'"
+  unfolding It_defs G'_def by auto
 
 lemma delta_ipda [simp]:
   "delta M = (\<lambda>q a s. case q of [X \<rightarrow> \<beta> . Tm a' # \<gamma>] \<Rightarrow> 
-            if a' = a then let r = [X \<rightarrow> \<beta> @ [Tm a] . \<gamma>] in {(r, [s])} else {} | _ \<Rightarrow> {})"
-using ipda unfolding IPDA_def by simp
-
-lemma delta_eps_ipda [simp]:
-  "delta_eps M = (\<lambda>q s. case (q,s) of 
-      ([X \<rightarrow> \<beta> . Nt Y # \<gamma>], _) \<Rightarrow> {([Y \<rightarrow> [] . \<alpha>], [X \<rightarrow> \<beta> . Nt Y#\<gamma>]#[s]) |\<alpha>. (Y,\<alpha>) \<in> Prods G'} |
-      ([Y \<rightarrow> \<alpha> . []], [X \<rightarrow> \<beta> . Nt Y' # \<gamma>]) 
-        \<Rightarrow> if Y = Y' then {([X \<rightarrow> \<beta>@[Nt Y] . \<gamma>], [])} else {} | _ \<Rightarrow> {})"
-  using ipda unfolding IPDA_def by simp
+            if a' = a \<and> (X, \<beta> @ Tm a' # \<gamma>) \<in> Prods G' then let r = [X \<rightarrow> \<beta> @ [Tm a] . \<gamma>] in {(r, [s])} 
+  else {} | _ \<Rightarrow> {})"
+  using ipda unfolding IPDA_def by (meson select_convs(4))
 
 
 lemma delta_Tm_neq_empty [simp]:
@@ -74,38 +73,125 @@ lemma delta_Tm_neq_empty [simp]:
 
 lemma delta_nempty_imp_Tm_eq:
   assumes "delta M p a q \<noteq> {}"
-  obtains X \<beta> \<gamma> where "p = [X \<rightarrow> \<beta> . Tm a # \<gamma>]"
+  obtains X \<beta> \<gamma> where "p = [X \<rightarrow> \<beta> . Tm a # \<gamma>]" "(X, \<beta> @ Tm a # \<gamma>) \<in> Prods G'"
 proof -
   obtain X \<beta> \<alpha> where p_def: "p = [X \<rightarrow> \<beta> . \<alpha>]" using item.exhaust by blast
   then consider (Nil) "\<alpha> = []" | (Tm_eq) \<gamma> where "\<alpha> = Tm a # \<gamma>" | 
    (Tm_neq) a' \<gamma> where "\<alpha> = Tm a' # \<gamma>" "a' \<noteq> a" | (Nt) A \<gamma> where "\<alpha> = Nt A # \<gamma>"
     using list.exhaust sym.exhaust by metis
-  then show thesis using p_def assms that by cases auto
+  then show thesis using p_def assms that by cases fastforce+
 qed
+
+corollary delta_nempty_imp_Tm_eq_Item:
+  assumes "delta M ([X \<rightarrow> \<beta> . Tm a # \<gamma>]) b q \<noteq> {}"
+  shows "(X, \<beta> @ Tm a # \<gamma>) \<in> Prods G'" "a = b"
+  using delta_nempty_imp_Tm_eq[OF assms] by blast+
+
+lemma in_prods_imp_delta_singleton [simp]:
+  assumes "(X, \<beta> @ Tm a # \<gamma>) \<in> Prods G'"
+  shows "delta M ([X \<rightarrow> \<beta> . Tm a # \<gamma>]) a q = {([X \<rightarrow> \<beta> @ [Tm a] . \<gamma>], [q])}"
+  using assms by auto
+
+lemma in_delta_imp_unchanged_prod:
+  assumes "(p, s) \<in> delta M q a r"
+  shows "prod_of_item p = prod_of_item q"
+proof (cases q)
+  case (Item X \<beta> \<gamma>)
+  then show ?thesis 
+  proof (cases \<gamma>)
+    case (Cons b \<delta>)
+    with assms Item have "(X, \<beta> @ Tm a # \<delta>) \<in> Prods G'" "Tm a = b"
+      using delta_nempty_imp_Tm_eq by blast+
+    then show ?thesis using in_prods_imp_delta_singleton Item Cons 
+      assms by auto
+  qed (use assms in simp)
+qed
+
+lemma delta_eps_ipda [simp]:
+  "delta_eps M = (\<lambda>q s. if prod_of_item q \<notin> Prods G' then {} else 
+    case (q,s) of 
+      ([X \<rightarrow> \<beta> . Nt Y # \<gamma>], _) \<Rightarrow> {([Y \<rightarrow> [] . \<alpha>], [X \<rightarrow> \<beta> . Nt Y#\<gamma>]#[s]) |\<alpha>. (Y,\<alpha>) \<in> Prods G'} |
+      ([Y \<rightarrow> \<alpha> . []], [X \<rightarrow> \<beta> . Nt Y' # \<gamma>]) 
+        \<Rightarrow> if Y = Y' \<and> (prod_of_item s \<in> Prods G')
+        then {([X \<rightarrow> \<beta>@[Nt Y] . \<gamma>], [])} else {} | _ \<Rightarrow> {})"
+  using ipda unfolding IPDA_def by (meson select_convs(5))
+
+lemma delta_eps_ipda_prods [simp]:
+  assumes "prod_of_item q \<in> Prods G'"
+  shows "delta_eps M q s = (case (q,s) of 
+      ([X \<rightarrow> \<beta> . Nt Y # \<gamma>], _) \<Rightarrow> {([Y \<rightarrow> [] . \<alpha>], [X \<rightarrow> \<beta> . Nt Y#\<gamma>]#[s]) |\<alpha>. (Y,\<alpha>) \<in> Prods G'} |
+      ([Y \<rightarrow> \<alpha> . []], [X \<rightarrow> \<beta> . Nt Y' # \<gamma>]) 
+        \<Rightarrow> if Y = Y' \<and> prod_of_item s \<in> Prods G' 
+        then {([X \<rightarrow> \<beta>@[Nt Y] . \<gamma>], [])} else {} | _ \<Rightarrow> {})"
+  using assms by auto
+
+lemma delta_eps_nempty_imp_prod:
+  assumes "delta_eps M q s \<noteq> {}"
+  shows "prod_of_item q \<in> Prods G'"
+  using assms by auto
 
 lemma delta_eps_Nt_neq_empty [simp]:
   assumes "Y \<noteq> Y'"
   shows "delta_eps M ([Y \<rightarrow> \<alpha> . []]) ([X \<rightarrow> \<beta> . Nt Y' # \<gamma>]) = {}"
-  using assms unfolding IPDA_def by simp
+  using assms by simp
+
+lemma delta_eps_complete_imp_snd_in_prods:
+  assumes "delta_eps M ([Y \<rightarrow> \<alpha> . []]) q \<noteq> {}"
+  shows "prod_of_item q \<in> Prods G'"
+proof -
+  note Y\<alpha>_prod = delta_eps_nempty_imp_prod[OF assms]
+  obtain X \<beta> \<gamma> where q_def: "q = [X \<rightarrow> \<beta> . \<gamma>]" using item.exhaust by metis
+  then show ?thesis
+  proof (cases \<gamma>)
+    case Nil
+    then show ?thesis using q_def assms 
+      by (smt (verit, ccfv_threshold) delta_eps_ipda_prods delta_eps_nempty_imp_prod item.case
+          list.simps(4) old.prod.case)
+  next
+    case (Cons a \<delta>)
+    then show ?thesis 
+    proof (cases a)
+      case (Nt A)
+      with Cons q_def have 
+        "delta_eps M ([Y \<rightarrow> \<alpha> . []]) q 
+          = (if Y = A \<and> prod_of_item q \<in> Prods G' then {([X \<rightarrow> \<beta> @ [Nt A] . \<delta>], [])} else {})"
+        using Y\<alpha>_prod by force
+      then show ?thesis using Cons q_def assms by argo
+    next
+      case (Tm b)
+      then show ?thesis using Cons q_def assms using Y\<alpha>_prod by auto
+    qed
+  qed
+qed
 
 
 lemma delta_eps_complete_imp_reducing:
   assumes "delta_eps M ([Y \<rightarrow> \<alpha> . []]) q \<noteq> {}"
-  obtains X \<beta> \<gamma> where "q = [X \<rightarrow> \<beta> . Nt Y # \<gamma>]"
+  obtains X \<beta> \<gamma> where "q = [X \<rightarrow> \<beta> . Nt Y # \<gamma>]" "(X, \<beta> @ Nt Y # \<gamma>) \<in> Prods G'" "(Y, \<alpha>) \<in> Prods G'"
 proof -
   obtain X \<beta> \<gamma> where q_def: "q = [X \<rightarrow> \<beta> . \<gamma>]" using item.exhaust by metis
   then show thesis
   proof (cases \<gamma>)
+    case Nil
+    then show ?thesis using assms q_def 
+      by (smt (verit, best) delta_eps_ipda item.case list.case(1) old.prod.case)
+  next
     case (Cons a as)
-    then show ?thesis 
-    by (cases a) (use assms q_def Cons that in fastforce)+
-  qed (use assms q_def in fastforce)
+    then show ?thesis       
+      using assms q_def Cons that delta_eps_ipda_prods delta_eps_complete_imp_snd_in_prods  
+      by (cases a)
+        (metis (lifting) append.right_neutral delta_eps_Nt_neq_empty delta_eps_ipda item.case,
+          smt (verit) case_prod_conv delta_eps_ipda item.case list.simps(4,5) sym.simps(6))
+  qed
 qed
+  
 
-lemma delta_eps_nempty_imp_expanding_or_reducing:
+
+lemma delta_eps_nempty_imp_expanding_or_reducing[consumes 1, case_names expanding reducing]:
   assumes "delta_eps M p q \<noteq> {}"
-  obtains X \<beta> Y \<gamma> where "p = [X \<rightarrow> \<beta> . Nt Y # \<gamma>]"  |
-    Y \<alpha> X \<beta>  \<gamma> where "p = [Y \<rightarrow> \<alpha> . []]" "q = [X \<rightarrow> \<beta> . Nt Y # \<gamma>]"
+  obtains X \<beta> Y \<gamma> where "p = [X \<rightarrow> \<beta> . Nt Y # \<gamma>]" "(X, \<beta> @ Nt Y # \<gamma>) \<in> Prods G'" |
+    Y \<alpha> X \<beta>  \<gamma> where "p = [Y \<rightarrow> \<alpha> . []]" "q = [X \<rightarrow> \<beta> . Nt Y # \<gamma>]" "(Y, \<alpha>) \<in> Prods G'" 
+      "(X, \<beta> @ Nt Y # \<gamma>) \<in> Prods G'"
 proof -
   obtain X \<alpha> \<beta> where p_def: "p = [X \<rightarrow> \<alpha> . \<beta>]" using item.exhaust by blast
   then show thesis
@@ -116,8 +202,19 @@ proof -
   next
     case (Cons a as)
     then show ?thesis 
-      by (cases a) (use p_def assms that in auto)
+      using p_def assms delta_eps_nempty_imp_prod that by (cases a)
+      (metis item.case, smt (verit, ccfv_threshold) case_prod_conv delta_eps_ipda item.case 
+        list.simps(5) sym.simps(6))
   qed
+qed
+
+lemma in_delta_eps_imp_in_prods:
+  assumes "(p, q) \<in> delta_eps M r s"
+  shows "prod_of_item p \<in> Prods G'"
+proof -
+  from assms have "delta_eps M r s \<noteq> {}" by blast
+  then show ?thesis
+    using assms by (cases rule: delta_eps_nempty_imp_expanding_or_reducing) auto
 qed
 
 lemmas init_defs = init_state_def init_symbol_def
@@ -126,6 +223,8 @@ lemma in_final_imp_final_state:
   assumes "q \<in> final_states M"
   shows "q = final_state"
   using assms unfolding IPDA_def S'_def S_def by simp
+
+section \<open>Step\<close>
 
 inductive step :: "('n,'t) item list \<times> 't list \<Rightarrow> ('n,'t) item list \<times> 't list 
                     \<Rightarrow> bool" (infix \<open>\<turnstile>\<close> 70) where
@@ -148,52 +247,56 @@ lemma step_len_dec:
   using step_equal_or_Cons[OF assms] by fastforce
 
 
-lemma shift [simp]:
-  "([A \<rightarrow> \<alpha> . Tm a # \<beta>]#\<rho>#\<rho>s, a#u) \<turnstile> ([A \<rightarrow> \<alpha>@[Tm a] . \<beta>]#\<rho>#\<rho>s, u)"
+lemma shifting_Cons [simp]:
+  assumes "(A, \<alpha> @ Tm a # \<beta>) \<in> Prods G'"
+  shows "([A \<rightarrow> \<alpha> . Tm a # \<beta>]#\<rho>#\<rho>s, a#u) \<turnstile> ([A \<rightarrow> \<alpha>@[Tm a] . \<beta>]#\<rho>#\<rho>s, u)"
 proof -
   have "([A \<rightarrow> \<alpha>@[Tm a] . \<beta>], [\<rho>]) \<in> delta M ([A \<rightarrow> \<alpha> . Tm a # \<beta>]) a \<rho>"
-    using IPDA_def by simp
+    using IPDA_def assms by simp
   then show ?thesis using delta 
     by (metis Cons_eq_appendI append.left_neutral)
 qed
 
 lemma shifting [simp]:
-  "([A \<rightarrow> \<alpha> . Tm a # \<beta>]#\<rho>@[init_symbol M], a#u) \<turnstile> ([A \<rightarrow> \<alpha>@[Tm a] . \<beta>]#\<rho>@[init_symbol M], u)"
-  by (cases \<rho>) auto
+  assumes "(A, \<alpha> @ Tm a # \<beta>) \<in> Prods G'"
+  shows "([A \<rightarrow> \<alpha> . Tm a # \<beta>]#\<rho>@[init_symbol M], a#u) \<turnstile> ([A \<rightarrow> \<alpha>@[Tm a] . \<beta>]#\<rho>@[init_symbol M], u)"
+  by (cases \<rho>) (use assms in auto)
 
 
 lemma reducing [simp]:
-  "([Y \<rightarrow> \<alpha> . []]#[X \<rightarrow> \<beta> . Nt Y#\<gamma>]#\<rho>, w) \<turnstile> ([X \<rightarrow> \<beta> @ [Nt Y] . \<gamma>]#\<rho>, w)"
+  assumes "(Y, \<alpha>) \<in> Prods G'" "(X, \<beta> @ Nt Y # \<gamma>) \<in> Prods G'"
+  shows "([Y \<rightarrow> \<alpha> . []]#[X \<rightarrow> \<beta> . Nt Y#\<gamma>]#\<rho>, w) \<turnstile> ([X \<rightarrow> \<beta> @ [Nt Y] . \<gamma>]#\<rho>, w)"
 proof -
   have "([X \<rightarrow> \<beta> @ [Nt Y] . \<gamma>], []) \<in> delta_eps M ([Y \<rightarrow> \<alpha> . []]) ([X \<rightarrow> \<beta> . Nt Y#\<gamma>])"
-    unfolding IPDA_def by simp
+    unfolding IPDA_def using assms by simp
   thus ?thesis using eps by (metis Cons_eq_appendI append.left_neutral)
 qed
 
 
 lemma expanding_in_delta_eps:
-  assumes "(Y, \<alpha>) \<in> Prods G'"
+  assumes "(Y, \<alpha>) \<in> Prods G'" "(X, \<beta> @ Nt Y # \<gamma>) \<in> Prods G'" 
   shows "([Y \<rightarrow> [] . \<alpha>], [[X \<rightarrow> \<beta> . Nt Y#\<gamma>], i]) \<in> delta_eps M ([X \<rightarrow> \<beta> . Nt Y#\<gamma>]) i"
-  using assms ipda unfolding G'_def S'_def S_def IPDA_def by auto
+  using assms ipda delta_eps_ipda_prods unfolding G'_def S'_def S_def IPDA_def  
+    by fastforce
+  
 
 lemma expanding_Cons [simp]:
-  assumes "(Y, \<alpha>) \<in> Prods G'"
+  assumes "(Y, \<alpha>) \<in> Prods G'" "(X, \<beta> @ Nt Y # \<gamma>) \<in> Prods G'" 
   shows "([X \<rightarrow> \<beta> . Nt Y#\<gamma>]#i#\<rho>, w) \<turnstile> ([Y \<rightarrow> [] . \<alpha>]#[X \<rightarrow> \<beta> . Nt Y#\<gamma>]#i#\<rho>, w)"
-  using expanding_in_delta_eps[OF assms] eps 
-  by (metis eq_Nil_appendI Cons_eq_appendI)
+  using expanding_in_delta_eps[OF assms] eps by (simp add: step.simps)
 
 lemma expanding:
-  assumes "(Y, \<alpha>) \<in> Prods G'"
+  assumes "(Y, \<alpha>) \<in> Prods G'" "(X, \<beta> @ Nt Y # \<gamma>) \<in> Prods G'"
   shows "([X \<rightarrow> \<beta> . Nt Y#\<gamma>]#\<rho>@[init_symbol M], w) \<turnstile> ([Y \<rightarrow> [] . \<alpha>]#[X \<rightarrow> \<beta> . Nt Y#\<gamma>]#\<rho>@[init_symbol M], w)"
-  using assms by (cases \<rho>) auto
+  using assms by (cases \<rho>) (auto simp: step.simps)
 
 lemma expanding_singleton:
-  assumes "Prods G' \<turnstile> [Nt Y] \<Rightarrow> \<alpha>"
+  assumes "Prods G' \<turnstile> [Nt Y] \<Rightarrow> \<alpha>" "(X, \<beta> @ Nt Y # \<gamma>) \<in> Prods G'"
   shows "([X \<rightarrow> \<beta> . Nt Y#\<gamma>]#\<rho>@[init_symbol M], w) \<turnstile> ([Y \<rightarrow> [] . \<alpha>]#[X \<rightarrow> \<beta> . Nt Y#\<gamma>]#\<rho>@[init_symbol M], w)"
   using assms expanding by (simp add: derive_singleton)
 
 lemma expanding_singleton_Cons:
-  assumes "Prods G' \<turnstile> [Nt Y] \<Rightarrow> \<alpha>"
+  assumes "Prods G' \<turnstile> [Nt Y] \<Rightarrow> \<alpha>" "(X, \<beta> @ Nt Y # \<gamma>) \<in> Prods G'"
   shows "([X \<rightarrow> \<beta> . Nt Y#\<gamma>]#i#\<rho>, w) \<turnstile> ([Y \<rightarrow> [] . \<alpha>]#[X \<rightarrow> \<beta> . Nt Y#\<gamma>]#i#\<rho>, w)"
   using assms expanding_Cons by (simp add: derive_singleton)
 
@@ -204,7 +307,7 @@ lemma in_delta_imp_shifting:
 proof -
   from assms have "delta M p0 a p1 \<noteq> {}" by auto
   from delta_nempty_imp_Tm_eq[OF this] 
-    obtain X \<beta> \<gamma> where p0_def: "p0 = [X \<rightarrow> \<beta> . Tm a # \<gamma>]" by blast
+    obtain X \<beta> \<gamma> where p0_def: "p0 = [X \<rightarrow> \<beta> . Tm a # \<gamma>]" "(X, \<beta> @ Tm a # \<gamma>) \<in> Prods G'" by blast
   hence "delta M p0 a p1 = {([X \<rightarrow> \<beta> @ [Tm a] . \<gamma>], [p1])}" by simp
   with assms show thesis using delta_ipda that p0_def 
     by (metis (lifting) singletonD)
@@ -213,19 +316,21 @@ qed
 lemma eps_cases[consumes 1, case_names reducing expand]:
   assumes "(q0,qs) \<in> delta_eps M p0 p1"
   obtains Y \<alpha> X \<beta> \<gamma> where
-    "p0 = [Y \<rightarrow> \<alpha> . []]" "p1 = [X \<rightarrow> \<beta> . Nt Y # \<gamma>]" "q0 = [X \<rightarrow> \<beta> @ [Nt Y] . \<gamma>]" "qs = []" |
+    "p0 = [Y \<rightarrow> \<alpha> . []]" "p1 = [X \<rightarrow> \<beta> . Nt Y # \<gamma>]" "q0 = [X \<rightarrow> \<beta> @ [Nt Y] . \<gamma>]" "qs = []" 
+    "(Y, \<alpha>) \<in> Prods G'" "(X, \<beta> @ Nt Y # \<gamma>) \<in> Prods G'" |
     X \<beta> Y \<gamma> \<alpha> where
     "p0 = [X \<rightarrow> \<beta> . Nt Y # \<gamma>]" "(Y, \<alpha>) \<in> Prods G'" "q0 = [Y \<rightarrow> [] . \<alpha>]" "qs = p0#[p1]" 
 proof -
   from delta_eps_nempty_imp_expanding_or_reducing consider 
-    X \<beta> Y \<gamma> where "p0 = [X \<rightarrow> \<beta> . Nt Y # \<gamma>]" |
-    Y \<alpha> X \<beta> \<gamma> where "p0 = [Y \<rightarrow> \<alpha> . []]" "p1 = [X \<rightarrow> \<beta> . Nt Y # \<gamma>]" 
+    X \<beta> Y \<gamma> where "p0 = [X \<rightarrow> \<beta> . Nt Y # \<gamma>]" "(X, \<beta> @ Nt Y # \<gamma>) \<in> Prods G'" |
+    Y \<alpha> X \<beta> \<gamma> where "p0 = [Y \<rightarrow> \<alpha> . []]" "p1 = [X \<rightarrow> \<beta> . Nt Y # \<gamma>]" "(Y, \<alpha>) \<in> Prods G'" 
+       "(X, \<beta> @ Nt Y # \<gamma>) \<in> Prods G'"
     using assms by blast
   then show thesis
     by cases (use that assms in auto) 
 qed
 
-lemma step_cases[consumes 1, case_names shift reduct expand, cases set: step]:
+lemma step_cases[consumes 1, case_names shift reduce expand, cases set: step]:
   assumes "c0 \<turnstile> c1"
 obtains A \<alpha> a \<beta> i \<rho> u where 
     "c0 = ([A \<rightarrow> \<alpha> . Tm a # \<beta>]#i#\<rho>, a#u)" "c1 = ([A \<rightarrow> \<alpha>@[Tm a] . \<beta>]#i#\<rho>, u)" |
@@ -233,7 +338,6 @@ obtains A \<alpha> a \<beta> i \<rho> u where
       "c0 = ([Y \<rightarrow> \<alpha> . []]#[X \<rightarrow> \<beta> . Nt Y#\<gamma>]#\<rho>, w)"  "c1 = ([X \<rightarrow> \<beta> @ [Nt Y] . \<gamma>]#\<rho>, w)" |
     Y \<alpha> X \<beta> \<gamma> i \<rho> w where 
     "c0 = ([X \<rightarrow> \<beta> . Nt Y#\<gamma>]#i#\<rho>, w)"  "c1 = ([Y \<rightarrow> [] . \<alpha>]#[X \<rightarrow> \<beta> . Nt Y#\<gamma>]#i#\<rho>, w)"
-      "(Y, \<alpha>) \<in> Prods G'"
   using assms proof cases
   case (delta \<alpha> p0 p1 \<alpha>' q qs a \<beta> w)
   from in_delta_imp_shifting[OF delta(5)] obtain X \<beta>' \<gamma> where "p0 = [X \<rightarrow> \<beta>' . Tm a # \<gamma>]" 
@@ -245,28 +349,80 @@ next
     by (cases rule: eps_cases) force+
 qed
 
-lemma step_imp_in_It:
-  assumes "i0 \<in> It G'" "i1 \<in> It G'"
-    "(i0#i1#is, u) \<turnstile> (j#js, v)"
-  shows "j \<in> It G'"
-  using assms(3,1,2) by (cases rule: step_cases) (simp add: It_defs)+
+lemma step_imp_in_prods:
+  assumes "(i # \<rho>, u) \<turnstile> (j # \<sigma>, v)"
+  shows "prod_of_item i \<in> Prods G' \<and> prod_of_item j \<in> Prods G'"
+  using assms proof (cases rule: step.cases)
+  case (delta \<alpha> p0 p1 \<alpha>' q qs a \<beta>)
+  then show ?thesis using delta_nempty_imp_Tm_eq in_delta_imp_unchanged_prod 
+    by (smt (verit, best) append_Cons empty_iff item.case list.inject)
+next
+  case (eps \<alpha> p0 p1 \<alpha>' q qs \<beta>)
+  then show ?thesis using in_delta_eps_imp_in_prods delta_eps_nempty_imp_prod 
+    by (metis (no_types, lifting) append_Cons equals0D list.inject)
+qed
+
+corollary step_imp_in_It:
+  assumes "(i # \<rho>, u) \<turnstile> (j # \<sigma>, v)"
+  shows "i \<in> It G'" "j \<in> It G'"
+  using step_imp_in_prods[OF assms] in_Prods_eq_in_It by auto
+
+lemma step_imp_not_Nil:
+  assumes "(\<rho>, u) \<turnstile> (\<sigma>, v)"
+  shows "\<rho> \<noteq> [] \<and> \<sigma> \<noteq> []"
+  using assms by cases auto
+
+lemma step_imp_two_items:
+  assumes "(\<rho>, u) \<turnstile> (\<sigma>, v)"
+  obtains i1 i2 \<tau> where "\<rho> = i1 # i2 # \<tau>" 
+  using assms by cases auto
 
 
-lemma Prods_G_closed_expanding:
+lemma step_app_init_symbol_preserved:
+  assumes "([A \<rightarrow> \<alpha> . \<beta>] # \<rho> @ [init_symbol M], u) \<turnstile> (\<sigma>, v)"
+    "[A \<rightarrow> \<alpha> . \<beta>] \<in> It G'"
+  obtains B \<gamma> \<delta> \<tau> where "\<sigma> = [B \<rightarrow> \<gamma> . \<delta>] # \<tau> @ [init_symbol M]"
+  using assms(1) proof cases
+  case (shift A \<alpha> a \<beta> i \<rho> u)
+  then show ?thesis using that by (metis list.inject prod.inject)
+next
+  case (reduce Y \<alpha> X \<beta> \<gamma> \<rho> w)
+  then show ?thesis using assms(2) that step_imp_in_It init_symbol_notin_It 
+    by (smt (verit, ccfv_SIG) append_eq_Cons_conv init_symbol_ipda item.inject list.discI 
+        list.inject prod.inject)
+next
+  case (expand Y \<alpha>' X \<beta>' \<gamma> i \<tau> w)
+  then show ?thesis using that[of _ _ _ "[A \<rightarrow> \<alpha> . \<beta>] # \<rho>"] by simp
+qed
+
+lemma expanding_imp_in_Prods_G:
   assumes "([X \<rightarrow> \<alpha> . Nt Y # \<beta>] # \<rho>, u) \<turnstile> ([Y \<rightarrow> [] . \<gamma>] # [X \<rightarrow> \<alpha> . Nt Y # \<beta>] # \<rho>, v)"
-    "(X, \<alpha> @ Nt Y # \<beta>) \<in> Prods G"
   shows "(Y, \<gamma>) \<in> Prods G"
-  using assms proof cases
-  case (expand Y \<alpha>' X \<beta>' \<gamma> i \<rho> w)
-  hence "(Y, \<alpha>') \<in> Prods G \<or> (Y, \<alpha>') = (S', [Nt S])" unfolding G'_def by auto
-  hence "(Y, \<alpha>') \<in> Prods G"
-  proof
-    assume "(Y, \<alpha>') = (S' , [Nt S])"
-    with assms(2) S'_Prod_notin_G(2)[of "\<alpha> @ Nt Y # \<beta>"] expand show ?thesis by simp
+proof -
+  from assms have "(Y, \<gamma>) \<in> Prods G'" using step_imp_in_prods by fastforce
+  then show ?thesis
+  proof (cases rule: G'_Prod_cases)
+    case init
+    with assms have "(X, \<alpha> @ Nt S' # \<beta>) \<in> Prods G'"
+      using step_imp_in_prods by fastforce
+    then show ?thesis using S'_Prod_notin_G' by simp
   qed simp
-  then show ?thesis using expand by blast
-qed simp+
+qed
 
+lemma step_not_expanding_unique:
+  assumes "(\<rho>, u) \<turnstile> c0" "(\<rho>, u) \<turnstile> c1"
+    "\<exists>X \<alpha> a \<beta>. hd \<rho> = [X \<rightarrow> \<alpha> . []] \<or> hd \<rho> = [X \<rightarrow> \<alpha> . Tm a # \<beta>]"
+  shows "c0 = c1"
+  using assms(1) by (cases; use assms(2) in cases, use assms(3) in auto)
+
+lemma step_reaches_final_imp_S:
+  assumes "([A \<rightarrow> \<alpha> . \<beta>] # \<rho> @ \<sigma>, u) \<turnstile> (final_state # \<sigma>, v)"
+  shows "([A \<rightarrow> \<alpha> . \<beta>] # \<rho> @ \<sigma>, u) = ([S \<rightarrow> \<alpha> . \<beta>] # init_state M # \<sigma>, v)"
+  using assms(1) by cases auto
+
+
+
+section \<open>Steps\<close>
 
 abbreviation steps (infix \<open>\<turnstile>*\<close> 50) where
   "steps \<equiv> (step \<^sup>*\<^sup>*)"
@@ -274,23 +430,30 @@ abbreviation steps (infix \<open>\<turnstile>*\<close> 50) where
 abbreviation stepn ( \<open>_ \<turnstile>'(_') _\<close> 50) where
   "stepn c0 n c1 \<equiv> (step ^^ n) c0 c1"
 
+lemma step_not_expanding_imp_reaches:
+  assumes "(\<rho>, u) \<turnstile> c0" "(\<rho>, u) \<turnstile>(Suc n) c1"
+    "\<exists>X \<alpha> a \<beta>. hd \<rho> = [X \<rightarrow> \<alpha> . []] \<or> hd \<rho> = [X \<rightarrow> \<alpha> . Tm a # \<beta>]"
+  shows "c0 \<turnstile>(n) c1"
+  using step_not_expanding_unique assms by (metis relpowp_Suc_D2)
+                                                         
 lemma steps_len_dec:
   "(p,u) \<turnstile>* (q,v) \<Longrightarrow> length u \<ge> length v" 
   by (induction "(p,u)" "(q,v)" arbitrary: q v rule: rtranclp.induct)
   (use step_len_dec surj_pair le_trans in fastforce)+
 
 lemma completes_Tms_Cons:
-  "([A \<rightarrow> \<alpha> . map Tm u @ \<beta>]#i#is, u@v) \<turnstile>* ([A \<rightarrow> \<alpha> @ map Tm u . \<beta>]#i#is, v)"
+  "(A, \<alpha> @ map Tm u @ \<beta>) \<in> Prods G' 
+    \<Longrightarrow> ([A \<rightarrow> \<alpha> . map Tm u @ \<beta>]#i#is, u@v) \<turnstile>* ([A \<rightarrow> \<alpha> @ map Tm u . \<beta>]#i#is, v)"
 proof (induction u arbitrary: \<alpha>)
   case (Cons a u)
-  have "([A \<rightarrow> \<alpha> . map Tm (a # u) @ \<beta>] # i # is, (a # u) @ v) 
+  hence "([A \<rightarrow> \<alpha> . map Tm (a # u) @ \<beta>] # i # is, (a # u) @ v) 
         \<turnstile> ([A \<rightarrow> \<alpha> @ [Tm a] . map Tm u @ \<beta>] # i # is, u @ v)"
     by simp
-  also note Cons[of "\<alpha>@[Tm a]"] 
-  finally show ?case by auto
+  also note Cons(1)[of "\<alpha>@[Tm a]"] 
+  finally show ?case using Cons by auto
 qed simp
 
-lemma stepn_Suc_imp_two_items:
+lemma stepn_Suc_imp_x:
   assumes "(\<rho>, u) \<turnstile>(Suc n) (\<sigma>, v)"
   obtains i j \<tau> where "\<rho> = i # j # \<tau>"
 proof -
@@ -307,12 +470,43 @@ proof -
   from assms obtain c where "(\<rho>, u) \<turnstile> c" 
     by (metis converse_rtranclpE prod.inject)
   then show thesis
-    using that by cases auto
+    using that step_imp_two_items prod.exhaust by metis
 qed
 
 lemma completes_Tms:
-  "([A \<rightarrow> \<alpha> . map Tm u @ \<beta>]#\<rho>@[init_symbol M], u@v) \<turnstile>* ([A \<rightarrow> \<alpha> @ map Tm u . \<beta>]#\<rho>@[init_symbol M], v)"
+  "(A, \<alpha> @ map Tm u @ \<beta>) \<in> Prods G' \<Longrightarrow> ([A \<rightarrow> \<alpha> . map Tm u @ \<beta>]#\<rho>@[init_symbol M], u@v) 
+                                          \<turnstile>* ([A \<rightarrow> \<alpha> @ map Tm u . \<beta>]#\<rho>@[init_symbol M], v)"
   using completes_Tms_Cons by (cases \<rho>) auto
+
+lemma steps_in_It:
+  "\<lbrakk>(i # \<rho>, u) \<turnstile>* (j # \<sigma>, v); i \<in> It G'\<rbrakk> \<Longrightarrow> j \<in> It G'"
+  by (induction "j # \<sigma>" v arbitrary: j \<sigma> rule: rtranclp_induct2)
+    (simp, metis neq_Nil_conv step_imp_in_It(2) step_imp_not_Nil)
+
+corollary steps_Suc_in_It:
+  assumes "(i # \<rho>, u) \<turnstile>(Suc n) (j # \<sigma>, v)"
+  shows  "i \<in> It G'" "j \<in> It G'"
+proof -
+  from assms obtain c where "(i # \<rho>, u) \<turnstile> c" 
+    by (metis relpowp_Suc_D2)
+  with step_imp_in_It(1) show "i \<in> It G'" 
+    by (smt (verit, ccfv_threshold) step_cases)
+  with assms[THEN relpowp_imp_rtranclp] show "j \<in> It G'"
+    using steps_in_It by simp
+qed
+
+
+corollary steps_neq_in_It:
+  assumes "(i # \<rho>, u) \<turnstile>* (j # \<sigma>, v)" "(i # \<rho>, u) \<noteq> (j # \<sigma>, v)"
+  shows "i \<in> It G' \<and> j \<in> It G'"
+  using assms(1) proof (cases rule: converse_rtranclpE)
+  case (step y)
+  from this(1) step_imp_in_It(1) have "i \<in> It G'" 
+    by (metis list.exhaust old.prod.exhaust step_imp_not_Nil)
+  then show ?thesis using steps_in_It step assms(1) by blast
+qed (use assms(2) in simp)
+
+
 
 lemma reachable_imp_in_It:
   "\<lbrakk>([init_state M, init_symbol M], u) \<turnstile>* (\<rho>, v); i \<in> set \<rho> - {init_symbol M}\<rbrakk> 
@@ -320,7 +514,7 @@ lemma reachable_imp_in_It:
 proof (induction arbitrary: i rule: rtranclp_induct2)
   case (step \<rho>0 u \<rho>1 v)
   from step(2) show ?case 
-    using step(3,4) by (cases rule: step_cases) (fastforce simp: It_defs)+ 
+    using steps_in_It step step_imp_in_It(2) by cases auto
 qed (auto simp: It_defs G'_def)
 
 lemma reachable_imp_not_Nil:
@@ -331,20 +525,8 @@ lemma reachable_imp_not_Nil:
 lemma reachable_imp_hd_not_init_symbol:
   assumes "([init_state M, init_symbol M], u) \<turnstile>* (i#\<rho>, v)"
   shows "i \<noteq> init_symbol M"
-proof -
-  from assms obtain n where "([init_state M, init_symbol M], u) \<turnstile>(n) (i#\<rho>, v)"
-    using rtranclp_imp_relpowp by fast
-  then show ?thesis
-  proof (induction n arbitrary: i \<rho> v)
-    case (Suc n)
-    then obtain j \<sigma> w where n_steps: "([init_state M, init_symbol M], u) \<turnstile>(n) (j#\<sigma>, w)"
-      "(j#\<sigma>, w) \<turnstile> (i#\<rho>, v)" using reachable_imp_not_Nil 
-      by (metis neq_Nil_conv relpowp_Suc_E rtranclp_power surj_pair)
-    with Suc have j_not_init: "j \<noteq> init_symbol M" by fast
-    from n_steps(2) show ?case 
-      by cases (use in_Prods_imp_item_neq_init_symbol in force)+
-  qed force
-qed
+  using assms steps_Suc_in_It init_symbol_notin_It  
+    by (cases rule: rtranclp.cases) (simp, meson relpowp_Suc_I rtranclp_power)
 
 corollary reachable_imp_head_in_It:
   "([init_state M, init_symbol M], u) \<turnstile>* (i#\<rho>, v) \<Longrightarrow> i \<in> It G'"
@@ -374,14 +556,18 @@ lemma init_state_expands[elim]:
   using assms proof cases
   case (expand Y \<alpha> X \<beta> \<gamma> i \<rho> w)
   then show ?thesis 
-    using G'_def S_neq_S' that by auto
+    using G'_def S_neq_S' that assms by auto
 qed auto
 
-lemma final_state_step_impossible:
-  assumes "([[S' \<rightarrow> \<alpha> . []], init_symbol M], u) \<turnstile> c"
+lemma complete_S'_step_impossible:
+  assumes "([[S' \<rightarrow> \<alpha> . []], init_symbol M], w) \<turnstile> c"
   shows False
   using assms by cases simp+
-  
+
+corollary complete_S'_steps_refl:
+  assumes "([[S' \<rightarrow> \<alpha> . []], init_symbol M], w) \<turnstile>* c"
+  shows "([[S' \<rightarrow> \<alpha> . []], init_symbol M], w) = c"
+  using assms complete_S'_step_impossible by (cases rule: converse_rtranclpE) auto
 
 
 lemma reachable_imp_init_or_in_G:
@@ -406,7 +592,7 @@ proof -
     proof (cases \<tau>)
       case Nil
       with \<tau>_def n_steps(2) have \<sigma>_init: "\<sigma> = [init_state M, init_symbol M]"
-        using final_state_step_impossible[of "[Nt S]"] append_eq_Cons_conv by fastforce 
+        using complete_S'_step_impossible[of "[Nt S]"] append_eq_Cons_conv by fastforce 
       with n_steps init_state_expands show ?thesis 
         using Suc.prems(2)[of _ "[]" "[Nt S]"] \<sigma>_init by force
     next
@@ -418,11 +604,7 @@ proof -
         moreover with Cons have
           "\<rho> = [Y \<rightarrow> [] . \<alpha>'] # \<tau> @ [[S' \<rightarrow> \<alpha> . \<beta>], init_symbol M]" by simp
         moreover from expand \<tau>_def Cons have "\<forall>i\<in>set ([Y \<rightarrow> [] . \<alpha>'] # \<tau>). ?in_Prods i" 
-        proof -
-          from expand \<tau>_def Cons have "(X, \<beta>' @ Nt Y # \<gamma>) \<in> Prods G" by auto
-          from Prods_G_closed_expanding[OF _ this] expand n_steps(2) \<tau>_def(3) show ?thesis 
-            by (metis append_Nil expanding_Cons item.case set_ConsD)
-        qed
+          using \<sigma>_def  expanding_imp_in_Prods_G expand n_steps(2) \<tau>_def(3) by auto
         ultimately show ?thesis using Suc.prems(2) \<tau>_def Cons by fastforce
       qed (cases \<nu>, (use \<tau>_def Cons Suc in auto))+
     qed
@@ -443,7 +625,7 @@ proof -
   moreover with step obtain r rs where 
     "ps = r#rs" "(r, rs) \<in> delta_eps M (init_state M) (init_symbol M)"
     using step_epsE by fastforce 
-  ultimately show thesis using that by auto
+  ultimately show thesis using that by blast
 qed
 
 corollary reachable_snd_not_empty_imp_hd_in_G:
@@ -463,48 +645,52 @@ qed
 
 lemma singleton_derive_imp_completes:
   assumes "Prods G' \<turnstile> [Nt X] \<Rightarrow> map Tm u"
+    "(A, \<alpha> @ Nt X # \<beta>) \<in> Prods G'"
   shows "([A \<rightarrow> \<alpha> . [Nt X] @ \<beta>] # \<rho> @ [init_symbol M], u @ v) 
           \<turnstile>* ([A \<rightarrow> \<alpha> @ [Nt X] . \<beta>] # \<rho> @ [init_symbol M], v)"
 proof -
-  from assms derive_singleton[of "Prods G'" "Nt X" "map Tm u"] expanding have 
+  note deriv = derive_singleton[of "Prods G'" "Nt X" "map Tm u"]
+  with assms expanding have 
     "([A \<rightarrow> \<alpha> . [Nt X] @ \<beta>] # \<rho> @ [init_symbol M], u @ v) 
       \<turnstile> ([X \<rightarrow> [] . map Tm u] # [A \<rightarrow> \<alpha> . [Nt X] @ \<beta>] # \<rho> @ [init_symbol M], u @ v)"
     by auto
-  also from completes_Tms have 
+  also with completes_Tms step_imp_in_prods have 
     "... \<turnstile>* ([X \<rightarrow> map Tm u . []] # [A \<rightarrow> \<alpha> . [Nt X] @ \<beta>] # \<rho> @ [init_symbol M], v)" 
-    by (metis append.right_neutral append_Nil completes_Tms_Cons)
-  also have "... \<turnstile> ([A \<rightarrow> \<alpha> @ [Nt X] . \<beta>] # \<rho> @ [init_symbol M], v)"
-    by simp
+    by (metis deriv append.right_neutral append_Nil assms(1) completes_Tms_Cons sym.inject(1))
+  also  have "... \<turnstile> ([A \<rightarrow> \<alpha> @ [Nt X] . \<beta>] # \<rho> @ [init_symbol M], v)"
+    using assms deriv by auto
   finally show ?thesis .
 qed
 
 
 lemma derive_imp_completes:
   assumes "Prods G' \<turnstile> \<beta> \<Rightarrow> map Tm w"
+    "(A, \<alpha> @ \<beta> @ \<gamma>) \<in> Prods G'"
   shows "([A \<rightarrow> \<alpha> . \<beta>@\<gamma>] # \<rho> @ [init_symbol M], w @ x) \<turnstile>* ([A \<rightarrow> \<alpha>@\<beta> . \<gamma>] # \<rho> @ [init_symbol M], x)"
 proof -
-  from derive_decomp[OF assms] obtain u v X y where \<beta>_decomp:
+  from derive_decomp[OF assms(1)] obtain u v X y where \<beta>_decomp:
     "\<beta> = map Tm u @ Nt X # map Tm y" "Prods G' \<turnstile> [Nt X] \<Rightarrow> map Tm v" "w = u @ v @ y" by metis
   with completes_Tms[of A \<alpha> u "Nt X # map Tm y @ \<gamma>" _ "v @ y @ x"] have 
     "([A \<rightarrow> \<alpha> . \<beta> @ \<gamma>] # \<rho> @ [init_symbol M], w @ x) 
       \<turnstile>* ([A \<rightarrow> \<alpha> @ map Tm u . Nt X # map Tm y @ \<gamma>] # \<rho> @ [init_symbol M], v @ y @ x)" 
-    by simp
+    using assms by simp
   also from singleton_derive_imp_completes[OF \<beta>_decomp(2), of _ "\<alpha> @ map Tm u" _ _ "y@x"] have 
     "... \<turnstile>* ([A \<rightarrow> \<alpha> @ map Tm u @ [Nt X] . map Tm y @ \<gamma>] # \<rho> @ [init_symbol M], y @ x)"
-    by simp
+    using \<beta>_decomp(1) assms(2) by auto
   also from completes_Tms have "... \<turnstile>* ([A \<rightarrow> \<alpha> @ \<beta> . \<gamma>] # \<rho> @ [init_symbol M], x)"
-    using \<beta>_decomp by (smt (verit, best) append.assoc append_Cons append_Nil)
+    using \<beta>_decomp by (smt (verit) append.assoc append_Cons append_Nil assms(2))
   finally show ?thesis .
 qed
 
 
 lemma derives_imp_completes:
   assumes "Prods G' \<turnstile> \<beta> \<Rightarrow>* map Tm w"
+    "(A, \<alpha> @ \<beta> @ \<gamma>) \<in> Prods G'"
   shows "([A \<rightarrow> \<alpha> . \<beta>@\<gamma>] # \<rho> @ [init_symbol M], w @ x) \<turnstile>* ([A \<rightarrow> \<alpha>@\<beta> . \<gamma>] # \<rho> @ [init_symbol M], x)"
 proof -
   from assms obtain n where "Prods G' \<turnstile> \<beta> \<Rightarrow>(n) map Tm w" 
     using rtranclp_imp_relpowp by fast
-  then show ?thesis
+  with assms(2) show ?thesis
   proof (induction n arbitrary: \<beta> w A \<alpha> \<gamma> \<rho> x rule: less_induct)
     case (less n)
     then show ?case 
@@ -512,28 +698,28 @@ proof -
       case (Suc m)
       note Suc_m = this
       with derives_decomp_less obtain \<delta>\<^sub>1 i u X j v \<delta>\<^sub>2 k y where
-        decomp:
+        \<beta>_decomp:
         "\<beta> = \<delta>\<^sub>1 @ Nt X # \<delta>\<^sub>2"
         "Prods G' \<turnstile> \<delta>\<^sub>1 \<Rightarrow>(i) map Tm u" "Prods G' \<turnstile> [Nt X] \<Rightarrow>(j) map Tm v" "Prods G' \<turnstile> \<delta>\<^sub>2 \<Rightarrow>(k) map Tm y"
         "w = u @ v @ y" "i + j + k = n" "j > 0" 
-        using less(2)  by (smt (verit, best))
+        using less(3)  by (smt (verit, best))
       hence leqs: "i < n" "k < n" by auto
       have first: "([A \<rightarrow> \<alpha> . \<beta> @ \<gamma>] # \<rho> @ [init_symbol M], w @ x) 
               \<turnstile>* ([A \<rightarrow> \<alpha> @ \<delta>\<^sub>1 . Nt X # \<delta>\<^sub>2 @ \<gamma>] # \<rho> @ [init_symbol M], v @ y @ x)"
         (is "_ \<turnstile>* (?\<sigma>, _)")
-        using less(1)[OF leqs(1) decomp(2), of _ _ "Nt X # \<delta>\<^sub>2 @ \<gamma>" _ "v @ y @ x"]
-          decomp by simp
+        using less(1)[OF leqs(1) _ \<beta>_decomp(2), of _ _ "Nt X # \<delta>\<^sub>2 @ \<gamma>" _ "v @ y @ x"]
+          \<beta>_decomp less.prems(1) by simp
       have last: "([A \<rightarrow> \<alpha> @ \<delta>\<^sub>1 @ [Nt X] . \<delta>\<^sub>2 @ \<gamma>] # \<rho> @ [init_symbol M], y @ x) 
                   \<turnstile>* ([A \<rightarrow> \<alpha> @ \<beta> . \<gamma>] # \<rho> @ [init_symbol M], x)"
-        using less(1)[OF leqs(2) decomp(4), of _ "\<alpha> @ \<delta>\<^sub>1 @ [Nt X]"] decomp(1) by simp
+        using less(1)[OF leqs(2) _ \<beta>_decomp(4), of _ "\<alpha> @ \<delta>\<^sub>1 @ [Nt X]"] \<beta>_decomp(1) less.prems(1) by simp
       show ?thesis 
       proof (cases "j = n")
         case True
-        with decomp have Tms: "i = 0" "k = 0" "\<delta>\<^sub>1 = map Tm u" "\<delta>\<^sub>2 = map Tm y"
+        with \<beta>_decomp have Tms: "i = 0" "k = 0" "\<delta>\<^sub>1 = map Tm u" "\<delta>\<^sub>2 = map Tm y"
           by auto
-        from True decomp(6,7) Suc obtain \<beta>' where m_steps:
+        from True \<beta>_decomp(6,7) Suc obtain \<beta>' where m_steps:
           "Prods G' \<turnstile> [Nt X] \<Rightarrow> \<beta>'" "Prods G' \<turnstile> \<beta>' \<Rightarrow>(m) map Tm v"
-          using decomp(3) by (meson relpowp_Suc_D2)
+          using \<beta>_decomp(3) by (meson relpowp_Suc_D2)
         show ?thesis 
         proof (cases m)
           case (Suc m')
@@ -547,34 +733,42 @@ proof -
             "Prods G' \<turnstile> [Nt Y] \<Rightarrow> \<gamma>'" "Prods G' \<turnstile> \<gamma>' \<Rightarrow>(j'') map Tm v'"
             "j'' < n"
             using \<beta>'_decomp(7) by (metis order_less_trans)
-          note first
-          also from m_steps \<beta>'_decomp(1) have 
+          hence Y_prod': "(Y, \<gamma>') \<in> Prods G'" using derive_singleton 
+            by (metis sym.inject(1))
+          from m_steps \<beta>'_decomp(1) have X_step: "(X, \<xi>\<^sub>1 @ Nt Y # \<xi>\<^sub>2) \<in> Prods G'" 
             "([A \<rightarrow> \<alpha> @ \<delta>\<^sub>1 . Nt X # \<delta>\<^sub>2 @ \<gamma>] # \<rho> @ [init_symbol M], v @ y @ x) 
-              \<turnstile> ([X \<rightarrow> [] . \<xi>\<^sub>1 @ Nt Y # \<xi>\<^sub>2] # ?\<sigma>, v @ y @ x)"
-            using expanding_singleton by simp
-          also from less(1)[OF \<beta>'_decomp(6,2), of _ _ _ _ "v' @ y' @ y @ x"] 
+              \<turnstile> ([X \<rightarrow> [] . \<xi>\<^sub>1 @ Nt Y # \<xi>\<^sub>2] # ?\<sigma>, v @ y @ x)" 
+            using expanding_singleton \<beta>_decomp(1) less.prems(1) by 
+              (metis derive_singleton sym.inject(1), force)
+          note first
+          also note X_step(2)
+          also from less(1)[OF \<beta>'_decomp(6) _ \<beta>'_decomp(2), of _ _ _ _ "v' @ y' @ y @ x"] 
           have "... \<turnstile>* ([X \<rightarrow> \<xi>\<^sub>1 . Nt Y # \<xi>\<^sub>2] # ?\<sigma>, v' @ y' @ y @ x)" 
                (is "_ \<turnstile>* (?\<tau>, _)")
+          using \<beta>'_decomp(5) append.assoc append_Cons append_Nil X_step(1)
             by (metis \<beta>'_decomp(5) append.assoc append_Cons append_Nil)
-          also from Y_prod(1) have "... \<turnstile> ([Y \<rightarrow> [] . \<gamma>'] # ?\<tau>, v' @ y' @ y @ x)" 
-            using expanding_singleton by fastforce
-          also from less(1)[OF Y_prod(3,2), of Y "[]" "[]" _ "y' @ y @ x"]
+          also with Y_prod' have "... \<turnstile> ([Y \<rightarrow> [] . \<gamma>'] # ?\<tau>, v' @ y' @ y @ x)" 
+             using X_step(1) by simp
+          also from less(1)[OF Y_prod(3) _ Y_prod(2), of Y "[]" "[]" _ "y' @ y @ x"]
           have "... \<turnstile>* ([Y \<rightarrow> \<gamma>' . []] # ?\<tau>, y' @ y @ x)" 
-            by (smt (verit, best) Cons_eq_appendI append.right_neutral self_append_conv2)
+            using Y_prod' 
+            by (smt (verit, best) Cons_eq_appendI self_append_conv self_append_conv2)
           also have "... \<turnstile> ([X \<rightarrow> \<xi>\<^sub>1 @ [Nt Y] . \<xi>\<^sub>2] # ?\<sigma>, y' @ y @ x)"
-            using reducing by presburger
-          also from less(1)[OF \<beta>'_decomp(8,4), of X _ "[]" _ "y @ x"] have
+            using reducing Y_prod' X_step(1) by presburger
+          also from less(1)[OF \<beta>'_decomp(8) _ \<beta>'_decomp(4), of X _ "[]" _ "y @ x"] have
             "... \<turnstile>* ([X \<rightarrow> \<beta>' . []] # ?\<sigma>, y @ x)"
-            using \<beta>'_decomp(1) append.assoc by (metis append.right_neutral append_Cons append_Nil)
-          finally show ?thesis using reducing last 
-            by (smt (verit, best) append_eq_appendI converse_rtranclp_into_rtranclp rtranclp_trans)
-        qed (use derive_imp_completes decomp Tms Suc_m less.prems relpowp_Suc_0 in metis)
+            using \<beta>'_decomp(1) append.assoc X_step(1) 
+            by (metis append.right_neutral append_Cons append_Nil)
+          finally show ?thesis using reducing last X_step(1) \<beta>'_decomp less.prems(1) \<beta>_decomp
+            by (smt (verit) append.assoc append_Cons converse_rtranclp_into_rtranclp 
+                derive_singleton m_steps(1) rtranclp_trans sym.inject(1))
+        qed (use derive_imp_completes \<beta>_decomp Tms Suc_m less.prems relpowp_Suc_0 in metis)
       next
         case False
-        hence "j < n" using decomp by linarith
+        hence "j < n" using \<beta>_decomp by linarith
         then show ?thesis
-          using first last derivern_singleton_imp_prod[OF decomp(3)]
-          by (smt (verit, ccfv_threshold) append.assoc append_Cons append_Nil decomp(3) less.IH
+          using first last derivern_singleton_imp_prod[OF \<beta>_decomp(3)] less.prems(1)
+          by (smt (verit, ccfv_threshold) \<beta>_decomp(1,3) append.assoc append_Cons append_self_conv2 less.IH
               rtranclp_trans)
       qed
     qed (use completes_Tms in simp)
@@ -583,23 +777,25 @@ qed
 
 
 
+lemma reaches_without_stack_imp_S':
+  assumes "([[A \<rightarrow> \<alpha> . \<beta>], init_symbol IPDA], w) \<turnstile>* ([final_state, init_symbol IPDA], [])"
+  shows "[A \<rightarrow> \<alpha> . \<beta>] = init_state M \<or> [A \<rightarrow> \<alpha> . \<beta>] = final_state"
+  sorry
+
+
+lemma reaches_final_imp_completes:
+  assumes "([A \<rightarrow> \<alpha> . \<beta>] # \<rho> @ [init_symbol IPDA], u) \<turnstile>* ([final_state, init_symbol IPDA], [])"
+  obtains v where 
+    "([A \<rightarrow> \<alpha> . \<beta>] # \<rho> @ [init_symbol IPDA], v) \<turnstile>* ([A \<rightarrow> \<alpha> @ \<beta> . []] # \<rho> @ [init_symbol IPDA], v)"
+    "([A \<rightarrow> \<alpha> @ \<beta> . []] # \<rho> @ [init_symbol IPDA], v) \<turnstile>* ([final_state, init_symbol IPDA], [])"
+  sorry
+
 definition Lang :: "'t list set" where
   "Lang \<equiv> {w. ([init_state M, init_symbol M], w) \<turnstile>* ([final_state, init_symbol M], [])}"
-
-
-lemma hist_singleton_init [simp]:
-  "hist ([[A \<rightarrow> \<alpha> . \<beta>], init_symbol M]) = \<alpha>"
-  unfolding IPDA_def using hist_singleton by auto
 
 lemma hist_init [simp]:
   "hist (\<rho> @ [init_symbol M]) = hist \<rho>"
   using IPDA_def by (induction \<rho>) auto
-
-lemma hd_in_prods_imp_derives_expanded_hist:
-  assumes "(Y, \<alpha>) \<in> P"
-  shows "P \<turnstile> hist ([X \<rightarrow> \<beta> @ [Nt Y] . \<gamma>] # \<rho>) \<Rightarrow>*  hist ([Y \<rightarrow> \<alpha> . []] # [X \<rightarrow> \<beta> . Nt Y # \<gamma>] # \<rho>)"         
-    (is "P \<turnstile> ?h1 \<Rightarrow>* ?h2")
-  using assms by (auto simp: derive_prepend derive_singleton r_into_rtranclp)
 
 
 lemma invariant: 
@@ -624,19 +820,19 @@ proof -
       moreover have "hist \<rho> = hist \<sigma> @ [Tm a]" using shift unfolding hist_defs by simp
       ultimately show ?thesis using derives_append[OF derives_x] u_decomp by simp
     next
-      case (reduct Y \<alpha> X \<beta> \<gamma> \<tau> x)
+      case (reduce Y \<alpha> X \<beta> \<gamma> \<tau> x)
       have "Prods G \<turnstile> hist \<rho> \<Rightarrow>* hist \<sigma>"
       proof -
-        from n_steps reduct have Y_prod: "(Y, \<alpha>) \<in> Prods G" 
+        from n_steps reduce have Y_prod: "(Y, \<alpha>) \<in> Prods G" 
           using reachable_snd_not_empty_imp_hd_in_G 
             relpowp_imp_rtranclp by fastforce
-        from reduct have "hist \<rho> = hist \<tau> @ \<beta> @ [Nt Y]" by simp
+        from reduce have "hist \<rho> = hist \<tau> @ \<beta> @ [Nt Y]" by simp
         also have "Prods G \<turnstile> ... \<Rightarrow>* hist \<tau> @ \<beta> @ \<alpha>"
           using Y_prod derives_prepend by (metis derive_singleton r_into_rtranclp) 
-        also have "... = hist \<sigma>" using reduct by auto
+        also have "... = hist \<sigma>" using reduce by auto
         finally show ?thesis .
       qed
-      also from reduct n_steps(1) Suc.IH have "Prods G \<turnstile> ... \<Rightarrow>* map Tm u" by blast
+      also from reduce n_steps(1) Suc.IH have "Prods G \<turnstile> ... \<Rightarrow>* map Tm u" by blast
       finally show ?thesis .
     next
       case (expand Y \<alpha> X \<beta> \<gamma> i \<tau> x)
@@ -648,7 +844,8 @@ qed
 corollary Lang_subst_Lang_G:
   "Lang \<subseteq> LangS G"
   unfolding Lang_def Context_Free_Grammar.Lang_def S_def 
-  by (standard, metis invariant append.right_neutral hist_singleton_init mem_Collect_eq)
+  by (standard, metis Nil_is_append_conv append.right_neutral hist_Cons hist_singleton
+    init_symbol_ipda invariant mem_Collect_eq)
 
 lemma Lang_G_subst_Lang: 
   "LangS G \<subseteq> Lang"
@@ -687,7 +884,6 @@ proof -
         Lang_eq_Lang_G Lang_preserved hist_singleton rtrancl_refl init_state_ipda ipda by force
   qed
 qed
-
 
 end
 
